a bug: IsMaxMinVersion is not shown on the tests panel

fatnode/stain.scala
@@ -1,0 +1,39 @@
+import stainless.lang._
+import stainless.collection._
+import stainless.annotation._
+
+object FatNode {
+
+  def slice(values: Array[Int], valuesVersions: Array[Int], 
+            lefts: Array[FatNode], leftsVersions: Array[Int],
+            rights: Array[FatNode], rightsVersions: Array[Int],
+            ValueSets:): List[A] = {
+    require(start >= 0 && end >= 0 && end <= array.length && end >= start)
+    decreases(end - start)
+    if (end - start == 0) Nil()
+    else Cons(array(start), slice(array, start + 1, end))
+  }
+
+  def arr = Array(1,2,3,4)
+
+  def test1 = {
+    slice(arr, 0, 4) == List(1,2,3,4)
+  }.holds
+
+  def test2 = {
+    slice(arr, 1, 4) == List(2,3,4)
+  }.holds
+
+  def test3 = {
+    slice(arr, 2, 4) == List(3,4)
+  }.holds
+
+  def test4 = {
+    slice(arr, 3, 4) == List(4)
+  }.holds
+
+  def test5 = {
+    slice(arr, 4, 4) == Nil[Int]()
+  }.holds
+
+}
